Finish postulation of ultrafilter lemma for Boolean Algebras i.e. BPIT.
On the way, develop a lot of basic theory of Boolean algebras,
introduce notation for its operations, construct adjoining of an
element to a filter, prove characterisation of maximal filters in
Boolean algebras.

src/Lattices.v
@@ -1,10 +1,13 @@
 Set Implicit Arguments. Unset Strict Implicit.
 
 Require Import Coq.Program.Basics.
+Require Import SetNotations.
 Require Import Coq.Classes.RelationClasses.
-(* Import Coq.Classes.RelationClasses (PreOrder, Equivalence). *)
+
+(* "Setoid handling" *)
 Require Coq.Classes.Morphisms. Import (notations) Coq.Classes.Morphisms.
 Import Coq.Classes.Morphisms (Proper).
+From Coq Require Setoid.
 
 (* Why is this missing? *)
 (* It caused an endless loop when searching for an instance of `Reflexive`
@@ -14,6 +17,8 @@ Import Coq.Classes.Morphisms (Proper).
 Structure Preordered :=
 { carrier :> Type; le : carrier -> carrier -> Prop; pre : PreOrder le }.
 
+(* In the context `X : Preordered`, we can use `le : X -> X -> Prop` without
+   specifying the implicit argument as `X`. *)
 Arguments le {X} : rename.
 
 Definition ge {X : Preordered} : X -> X -> Prop := flip le.
@@ -25,7 +30,7 @@ Notation "x ≤ y"      := (le x y)          (at level 70).
 Notation "x ≥[ X ] y" := (ge (X := X) x y) (at level 70).
 Notation "x ≥ y"      := (ge x y)          (at level 70).
 
-Section PreorderedProperties. Variables (X : Preordered).
+Section PreorderedProperties. Context {X : Preordered}.
 
 Definition le_refl : Reflexive X.(le) := reflexivity.
 Definition le_rfl {x : X} : x ≤ x := le_refl x.
@@ -34,17 +39,15 @@ Definition le_trans : Transitive X.(le) := transitivity.
 
 Definition equiv (x y : X) : Prop := x ≤ y /\ y ≤ x.
 
-Notation "x ∼ y" := (equiv x y) (at level 70).
-
-Section ProjectedIneqs. Variables (x y : X) (h : x ∼ y).
+Section ProjectedIneqs. Context [x y : X] (h : equiv x y).
 Definition equiv_le     : x ≤ y := proj1 h.
 Definition equiv_le_rev : y ≤ x := proj2 h.
 Definition equiv_ge     : x ≥ y := proj2 h.
 Definition equiv_ge_rev : y ≥ x := proj1 h.
 End ProjectedIneqs.
 
-Instance equiv_refl : Reflexive equiv := fun _ => conj le_rfl le_rfl.
-Definition equiv_rfl {x : X} : x ∼ x := equiv_refl x.
+Definition equiv_refl : Reflexive equiv := fun _ => conj le_rfl le_rfl.
+Definition equiv_rfl {x : X} : equiv x x := equiv_refl x.
 
 Definition equiv_sym : Symmetric equiv :=
 fun _ _ h => conj (equiv_le_rev h) (equiv_le h).
@@ -53,18 +56,17 @@ Definition equiv_trans : Transitive equiv := fun _ _ _ h1 h2 =>
 conj (le_trans (equiv_le h1) (equiv_le h2))
      (le_trans (equiv_le_rev h2) (equiv_le_rev h1)).
 
-Definition equiv_equivalence : Equivalence equiv :=
+Instance equiv_equivalence : Equivalence equiv :=
 Build_Equivalence equiv equiv_refl equiv_sym equiv_trans.
 
-Definition le_respects_equiv : Proper (equiv ==> equiv ==> iff) X.(le) :=
-fun x1 x2 h_x y1 y2 h_y => conj
+Instance le_respects_equiv : Proper (equiv ==> equiv ==> iff) X.(le) :=
+fun _ _ h_x _ _ h_y => conj
 (fun h_le_1 => le_trans (le_trans (equiv_ge h_x) h_le_1) (equiv_le h_y))
 (fun h_le_2 => le_trans (le_trans (equiv_le h_x) h_le_2) (equiv_ge h_y)).
 
 End PreorderedProperties.
-Arguments equiv {X}.
-(* Print le. Print le_refl. Print le_rfl. Print le_trans. Print equiv. *)
 
+Notation "x ∼ y" := (equiv x y) (at level 70).
 Notation "x ∼[ X ] y" := (equiv (X := X) x y) (at level 70).
 
 Definition Preordered_dual (X : Preordered) : Preordered := {|
@@ -75,94 +77,228 @@ Definition Preordered_dual (X : Preordered) : Preordered := {|
 
 Section SpecialElements.
 
-Definition is_sup (A : Subset
+(* Definition is_sup (A : Subset *)
 
 End SpecialElements.
 
 Structure BooleanAlgebra := {
-  carrier :> Preordered;
+  preCarrier :> Preordered;
 
-  and : carrier -> carrier -> carrier;
-  or : carrier -> carrier -> carrier;
-  true : carrier; false : carrier;
-  not : carrier -> carrier;
+  and : preCarrier -> preCarrier -> preCarrier;
+  or : preCarrier -> preCarrier -> preCarrier;
+  true : preCarrier; false : preCarrier;
+  not : preCarrier -> preCarrier;
 
-  and_spec {p q r} : le r (and p q) <-> le r p /\ le r q;
-  or_spec {p q r} : le (or p q) r <-> le p r /\ le q r;
-  false_spec {p} : le false p; true_spec {p} : le p true;
-  and_not_spec {p} : eq (and p (not p)) false;
-  or_not_spec {p} : eq (or p (not p)) true;
+  and_spec p q r : le r (and p q) <-> le r p /\ le r q;
+  or_spec p q r : le (or p q) r <-> le p r /\ le q r;
+  and_distrib_or p q r : equiv (and p (or q r)) (or (and p q) (and p r));
+  false_spec p : le false p; true_spec p : le p true;
+  and_not' p : and p (not p) ≤ false;
+  or_not' p : true ≤ or p (not p)
 }.
 
-Structure filter (B : BooleanAlgebra) := {
-  set :> Subset B.(carrier);
+Local Notation "⊥[ B ]" := (B.(false)).
+Local Notation "⊥"      := (_.(false)).
+Local Notation "⊤[ B ]" := (B.(true)).
+Local Notation "⊤"      := (_.(true)).
+(* I can redefine /\, \/, but I can't change their levels.  So use \./, /.\. *)
+Local Notation "x /.\[ B ] y" := (B.(and) x y) (at level 65, right associativity).
+Local Notation "x /.\ y"      := (_.(and) x y) (at level 65, right associativity).
+Local Notation "x \./[ B ] y" := (B.(or) x y)  (at level 65, right associativity).
+Local Notation "x \./ y"      := (_.(or) x y)  (at level 65, right associativity).
+Local Notation "¬ x"         := (_.(not) x)   (at level 35).
 
-  filter_true_spec : B.(true) ∈ set;
-  filter_false_spec : B.(false) ∉ set;
-  filter_mono p q : B.(le) p q -> p ∈ set -> q ∈ set;
-  filter_and_spec p q : p ∈ set -> q ∈ set -> B.(and) p q ∈ set;
-}.
+Section BasicResults. Context {B : BooleanAlgebra}.
 
-Section BasicResults.
-Variable (B : BooleanAlgebra).
+Definition false_of_le_false p (h : p ≤ ⊥) : p ∼ ⊥ := conj h (B.(false_spec) p).
+Definition true_of_true_le p (h : ⊤ ≤ p) : p ∼ ⊤ := conj (B.(true_spec) p) h.
 
-Definition le_refl : forall {p}, B.(le) p p := B.(is_preorder).(preord_refl _ _).
-Definition le_trans : forall p q r, B.(le) p q -> B.(le) q r -> B.(le) p r :=
-B.(is_preorder).(preord_trans _ _).
+Definition and_not_equiv_false p : p /.\ ¬p ∼ ⊥ := false_of_le_false (and_not' p).
+Definition or_not_equiv_true p : p \./ ¬p ∼ ⊤ := true_of_true_le (or_not' p).
 
-Definition and_le_left p q : B.(le) (B.(and) p q) p :=
-  proj1 (proj1 B.(and_spec) le_refl).
-Definition and_le_right p q : B.(le) (B.(and) p q) q :=
-  proj2 (proj1 B.(and_spec) le_refl).
+Definition binop_respects_equiv_of_mono (bin_op : B -> B -> B)
+        (h : Proper (le ==> le ==> le) bin_op)
+    : Proper (equiv ==> equiv ==> equiv) bin_op :=
+fun _ _ h_x _ _ h_y => conj (h _ _ (equiv_le h_x)     _ _ (equiv_le h_y))
+                            (h _ _ (equiv_le_rev h_x) _ _ (equiv_le_rev h_y)).
+
+Section and.
+
+Definition and_le_left p q : p /.\ q ≤ p :=
+proj1 (proj1 (B.(and_spec) p q (p /.\ q)) le_rfl).
+Definition and_le_right p q : p /.\ q ≤ q :=
+proj2 (proj1 (B.(and_spec) p q (p /.\ q)) le_rfl).
+Definition le_and_of_le_both p q r : r ≤ p -> r ≤ q -> r ≤ p /.\ q :=
+fun h1 h2 => proj2 (B.(and_spec) p q r) (conj h1 h2).
+
+Definition and_mono : Proper (le ++> le ++> le) B.(and) := fun x1 x2 h_x y1 y2 h_y =>
+le_and_of_le_both (le_trans (and_le_left x1 y1) h_x)
+                  (le_trans (and_le_right x1 y1) h_y).
+
+Instance and_respects_equiv : Proper (equiv ==> equiv ==> equiv) B.(and) :=
+binop_respects_equiv_of_mono and_mono.
+
+Definition and_true p : p /.\ ⊤ ∼ p :=
+conj (and_le_left p ⊤) (le_and_of_le_both (le_refl p) (B.(true_spec) p)).
+
+Definition and_false p : p /.\ ⊥ ∼ ⊥ :=
+conj (and_le_right p ⊥) (B.(false_spec) _).
+
+Definition and_comm p q : p /.\ q ∼ q /.\ p := conj
+(le_and_of_le_both (and_le_right p q) (and_le_left p q))
+(le_and_of_le_both (and_le_right q p) (and_le_left q p)).
+
+Definition and_assoc p q r : (p /.\ q) /.\ r ∼ p /.\ (q /.\ r) := conj
+(le_and_of_le_both   (le_trans (and_le_left _ r) (and_le_left p q)  : _ ≤ p)
+  (le_and_of_le_both (le_trans (and_le_left _ r) (and_le_right p q) : _ ≤ q)
+                     (and_le_right _ r                              : _ ≤ r)))
+(le_and_of_le_both (le_and_of_le_both
+  (and_le_left p _                                : _ ≤ p)
+  (le_trans (and_le_right p _) (and_le_left q r)  : _ ≤ q))
+  (le_trans (and_le_right p _) (and_le_right q r) : _ ≤ r)).
+
+End and.
+
+Section or.
+
+Definition left_le_or p q : p ≤ p \./ q :=
+proj1 (proj1 (B.(or_spec) p q (p \./ q)) le_rfl).
+Definition right_le_or p q : q ≤ p \./ q :=
+proj2 (proj1 (B.(or_spec) p q (p \./ q)) le_rfl).
+Definition or_le_of_both_le p q r : p ≤ r -> q ≤ r -> p \./ q ≤ r :=
+fun h1 h2 => proj2 (B.(or_spec) p q r) (conj h1 h2).
+
+Definition or_mono : Proper (le ++> le ++> le) B.(or) := fun x1 x2 h_x y1 y2 h_y =>
+or_le_of_both_le (le_trans h_x (left_le_or x2 y2))
+                 (le_trans h_y (right_le_or x2 y2)).
+
+Instance or_respects_equiv : Proper (equiv ==> equiv ==> equiv) B.(or) :=
+binop_respects_equiv_of_mono or_mono.
+
+Definition or_false p : p \./ ⊥ ∼ p :=
+conj (or_le_of_both_le (le_refl p) (B.(false_spec) p)) (left_le_or p ⊥).
+
+Definition or_true p : p \./ ⊤ ∼ ⊤ :=
+conj (B.(true_spec) _) (right_le_or p ⊤).
+
+Definition or_comm p q : p \./ q ∼ q \./ p := conj
+(or_le_of_both_le (right_le_or q p) (left_le_or q p))
+(or_le_of_both_le (right_le_or p q) (left_le_or p q)).
+
+Definition or_assoc p q r : (p \./ q) \./ r ∼ p \./ (q \./ r) := conj
+(or_le_of_both_le (or_le_of_both_le
+  (left_le_or p _                               : p ≤ _)
+  (le_trans (left_le_or q r) (right_le_or p _)  : q ≤ _))
+  (le_trans (right_le_or q r) (right_le_or p _) : r ≤ _))
+(or_le_of_both_le   (le_trans (left_le_or p q) (left_le_or _ r)  : p ≤ _)
+  (or_le_of_both_le (le_trans (right_le_or p q) (left_le_or _ r) : q ≤ _)
+                     (right_le_or _ r                            : r ≤ _))).
+
+End or.
+
+Definition or_distrib_and p q r : p \./[B] (q /.\ r) ∼ (p \./ q) /.\ (p \./ r).
+Admitted.
+
+(* Can't get setoid rewriting/etc. to work *)
+Definition le_of_and_false_of_or_true p q r (h1 : p /.\ q ∼ ⊥) (h2 : p \./ r ∼ ⊤)
+    : q ≤[ B ] r.
+apply (and_respects_equiv (equiv_refl q)) in h2.
+apply (equiv_trans (equiv_sym (and_distrib_or q p r))) in h2.
+apply (fun h => equiv_trans h (and_true q)) in h2.
+apply (equiv_trans (equiv_sym (or_respects_equiv (equiv_trans (and_comm q p) h1) (equiv_refl (q /.\ r))))) in h2.
+apply (equiv_trans (equiv_sym (equiv_trans (or_comm ⊥ _) (or_false _)))) in h2.
+apply (le_respects_equiv h2 equiv_rfl).
+exact (and_le_right q r).
+Defined.
+
+Definition le_not_of_and_false p q (h : p /.\ q ∼ ⊥) : q ≤ ¬p :=
+le_of_and_false_of_or_true h (or_not_equiv_true p).
+
+Definition not_le_of_or_true p q (h : p \./ q ∼ ⊤) : ¬p ≤ q :=
+le_of_and_false_of_or_true (and_not_equiv_false p) (h).
 
 End BasicResults.
-Arguments and_le_left {B p q}. Arguments and_le_right {B p q}.
 
-Section Ultrafilters.
-Variable (B : BooleanAlgebra) (f : filter B).
+Section Filters.
+Context (B : BooleanAlgebra).
 
-Definition filter_adjoin (p : B) (h : B.(not) p ∉ f) : filter B := {|
-  set := fun q => exists2 r, r ∈ f & B.(le) (B.(and) p r) q;
+Structure filter := {
+  filterSet :> unary_predicate B;
 
-  filter_true_spec := ex_intro2 _ (fun r => B.(le) (B.(and) p r) B.(true))
-                          B.(true) f.(filter_true_spec) B.(true_spec);
+  filter_true_spec : ⊤ ∈ filterSet;
+  filter_false_spec : ⊥ ∉ filterSet;
+  filter_mono p q : p ≤ q -> p ∈ filterSet -> q ∈ filterSet;
+  filter_and_spec p q : p ∈ filterSet -> q ∈ filterSet -> p /.\ q ∈ filterSet;
+}.
+
+#[local] Arguments ex_intro2 [A P Q].
+Definition filter_adjoin (f : filter) [p] (h : ¬p ∉ f) : filter := {|
+  filterSet := fun q => exists2 r, r ∈ f & p /.\ r ≤ q;
+
+  (* No idea why it guesses Q wrong when the expected type LITERALLY
+     specifies it. *)
+  filter_true_spec := ex_intro2 (Q := fun r => p /.\ r ≤ ⊤)
+                        ⊤ f.(filter_true_spec) (B.(true_spec) _);
   filter_false_spec h' := let (r, h_in, h_le) := h' in
-                          let h' : B.(le) r (B.(not) p) :=
-                            _ in
-    h (f.(filter_mono) h' h_in);
+    h (f.(filter_mono) (le_not_of_and_false (false_of_le_false h_le)) h_in);
 
   filter_mono q q' h_le h' := let (r, h_in, h_le') := h' in
-    ex_intro2 _ _ r h_in (le_trans h_le' h_le);
+    ex_intro2 r h_in (le_trans h_le' h_le);
 
-  filter_and_spec q q' h h' := let (r, h_in, h_le) := h in let (r', h_in', h_le') := h' in
-    ex_intro2 _ _ (B.(and) r r') (f.(filter_and_spec) h_in h_in')
-                  (let r_ := B.(and) p (B.(and) r r') in
-                   let h' : B.(le) r_ p := and_le_left in
-                   let h'' : B.(le) r_ r := le_trans and_le_right and_le_left in
-                   let h''' : B.(le) r_ r' := le_trans and_le_right and_le_right in
-                   let h : B.(le) r_ q := le_trans (proj2 B.(and_spec) (conj h' h'')) h_le in
-                   let h' : B.(le) r_ q' := le_trans (proj2 B.(and_spec) (conj h' h''')) h_le' in
-                   proj2 B.(and_spec) (conj h h'))
+  filter_and_spec q1 q2 h1 h2 :=
+    let (r1, h_in1, h_le1) := h1 in let (r2, h_in2, h_le2) := h2 in
+    ex_intro2 (r1 /.\ r2) (f.(filter_and_spec) h_in1 h_in2)
+      (let r := p /.\ (r1 /.\ r2) in
+       let h1 : r ≤ p /.\ r1 := and_mono le_rfl (and_le_left r1 r2) in
+       let h2 : r ≤ p /.\ r2 := and_mono le_rfl (and_le_right r1 r2) in
+       le_and_of_le_both (le_trans h1 h_le1) (le_trans h2 h_le2))
 |}.
 
-Definition maximal (B : BooleanAlgebra) (f : filter B) :=
-forall f' : filter B, f ⊆ f' -> f' ⊆ f.
+Definition filter_sub_adjoin (f : filter) p (h : ¬p ∉ f) : f ⊆ filter_adjoin h := fun q h' =>
+ex_intro2 (Q := fun r => p /.\ r ≤ q) q h' (and_le_right p q).
 
-Definition adjoin (B : Bool
+Definition in_filter_adjoin (f : filter) p (h : ¬p ∉ f) : p ∈ filter_adjoin h :=
+ex_intro2 ⊤ f.(filter_true_spec) (and_le_left p ⊤).
 
-Theorem maximal_iff_mem_or_mem_not B f : maximal f <-> forall p, (* p ∈ f \/ B.(not) p ∈ f *) B.(not) p ∉ f -> p ∈ f.
+Section Ultrafilters.
+Context (f : filter).
+
+Definition filter_maximal := forall f' : filter, f ⊆ f' -> f' ⊆ f.
+
+(* We use here lem in the form `forall p, p ∈ f \/ ¬p ∈ f`. *)
+Theorem filter_maximal_iff_mem_or_not_mem {h_em : forall p, p ∈ f \/ p ∉ f}
+    : filter_maximal <-> forall p, p ∈ f \/ ¬p ∈ f.
 split.
-- intros h_max p. 
+- intros h_max p.
+  destruct (h_em (¬p)) as [h_n_in|h_n_notin].
+  + exact (or_intror h_n_in).
+  + apply or_introl.
+    apply (h_max (filter_adjoin h_n_notin) (filter_sub_adjoin h_n_notin)).
+    exact (in_filter_adjoin h_n_notin).
+  (* destruct (h_em p) as [|h_notin], (h_em (¬p)) as [|h_nnotin]
+  ; try ((apply or_introl + apply or_intror); assumption).
+  (* remaining case: p ∉ f and ¬p ∉ f *)
+  exfalso.
+  exact (h_notin (h_max _ (filter_sub_adjoin h_nnotin)
+                          p (in_filter_adjoin h_nnotin))). *)
 - intros h f' h_incl p h_in_f'.
-  assert (h_nn_in_f' : B.(not) p ∉ f').
+  assert (h_n_notin' : ¬p ∉ f').
   { intro. apply f'.(filter_false_spec).
-    apply (f'.(filter_mono) (proj1 (B.(and_not_spec) p))).
+    apply (f'.(filter_mono) (equiv_le (and_not_equiv_false p))).
     apply (f'.(filter_and_spec) h_in_f').
     assumption. }
-  (* destruct (h p) as [h_p|h_np].
-  + exact h_p.
-  + contradiction (h_nn_in_f' (h_incl _ h_np)). *)
+  destruct (h p) as [h_p|h_np]. + exact h_p.
+  + contradiction (h_n_notin' (h_incl _ h_np)).
 Qed.
 
 End Ultrafilters.
 
+Definition Ultrafilter := {f : filter | filter_maximal f}.
+
+End Filters.
+
+
+Definition BPIT (B : BooleanAlgebra) :=
+forall f : filter B, exists2 f' : filter B, filter_maximal f' & f ⊆ f'.
+
+Axiom boolean_prime_ideal_theorem : forall B : BooleanAlgebra, BPIT B.
